crates/correctness/lean/MxxCorrectness/Generated/ToyExample/Ir.lean
@@ -8,11 +8,11 @@ def ToyExample_generatorVersion : String := "mxx-correctness-emitter-v9"
 
 def ToyExample_protocolSourcePaths : List String := ["crates/correctness/Cargo.toml", "crates/correctness/examples/emit_correctness.rs", "crates/correctness/src", "crates/dsl/Cargo.toml", "crates/dsl/src", "crates/ir-core/Cargo.toml", "crates/ir-core/src"]
 
-def ToyExample_protocolSourceHash : String := "601d8341ad2e0538d2695db3d1513999dfea8274bf78a362428c62a289f8e72b"
+def ToyExample_protocolSourceHash : String := "cd3b6802243142fcb152b83ffd9341500ed9252c581e4ef7297a5bca140e8273"
 
 def ToyExample_workflowHash : String := "eec6cc84a07b935c537fee71c5f133e7e371b21f39e3757def3b287cbf269635"
 
-def ToyExample_toolkitHash : String := "6cc0ac8a8fde258276356918581e7c33d163b6852ce426f4f298bda191672487"
+def ToyExample_toolkitHash : String := "e4363b6fbde2e342f934fe11ff3897bd7185a683b11a404bc00f18f9bb71234c"
 
 def ToyExample_derivationHash : String := "1eb7ee1d85bf85dc59fea9e4e198e1cfa94df8fd0bf8168d408a754514520933"
 
